src/Instr.v
@@ -31,44 +31,306 @@ Lemma auth_secure:
      >!} Auth t.
 Proof.
   unfold corr2; intros.
-  destruct_lift H; cleanup.
+  destruct_lift H1; cleanup.
   repeat inv_exec_perm; simpl in *; cleanup;
   try rewrite app_nil_r.
   {
-    edestruct H4; eauto.
+    edestruct H6; eauto.
     pred_apply; cancel; eauto.
     or_l; cancel.
   }
   {
-    edestruct H4; eauto.
+    edestruct H6; eauto.
     pred_apply; cancel; eauto.
     or_r; cancel.
   }
   split_ors; cleanup; inv_exec_perm;
   try rewrite app_nil_r.
   {
-    edestruct H4; eauto.
+    edestruct H6; eauto.
     pred_apply; cancel; eauto.
     or_l; cancel.
   }
   {
-    edestruct H4; eauto.
+    edestruct H6; eauto.
     pred_apply; cancel; eauto.
     or_r; cancel.
   }
   split_ors; cleanup; inv_exec_perm;
   try rewrite app_nil_r.
   {
-    edestruct H4; eauto.
+    edestruct H6; eauto.
     pred_apply; cancel; eauto.
     or_l; cancel.
   }
   {
-    edestruct H4; eauto.
+    edestruct H6; eauto.
     pred_apply; cancel; eauto.
     or_r; cancel.
   }
 Qed.
+
+Lemma mem_merges_to_none :
+  forall V1 V2 (bm: block_mem V1) (bt: block_mem V2) btb h,
+    (mem_merges_to (AEQ:= handle_eq_dec)) bt bm btb ->
+    (bt h = None \/ bm h = None) ->
+    btb h = None.
+Proof.
+  unfold mem_merges_to, memmatch; intros.
+  cleanup; specialize (H1 h).
+  destruct (btb h); intuition;
+    edestruct p, H1;
+    edestruct H3; eauto; congruence.
+Qed.
+
+Lemma mem_merges_to_upd:
+  forall V1 V2 (bm: block_mem V1) (bt: block_mem V2) btb h x1 x2,
+    (mem_merges_to (AEQ:= handle_eq_dec)) bt bm btb ->
+    (mem_merges_to (AEQ:= handle_eq_dec)) (upd bt h x1) (upd bm h x2) ((upd (AEQ:=handle_eq_dec)) btb h (x1,x2)).
+Proof.
+  unfold mem_merges_to, memmatch; intros.
+  cleanup.
+  split; intros.
+  {
+    split; intros.
+   all: destruct (handle_eq_dec h h0); subst;
+     [rewrite upd_eq in H1; eauto; congruence |
+      rewrite upd_ne in H1; eauto;
+      rewrite upd_ne; eauto;
+      apply H; eauto].
+  }
+  {
+    split; intros; cleanup.
+    destruct (handle_eq_dec h h0); subst;
+    [rewrite upd_eq in H1; eauto;
+     rewrite upd_eq in H2; eauto; cleanup;
+     apply upd_eq; eauto |
+     rewrite upd_ne in H1; eauto;
+     rewrite upd_ne in H2; eauto;
+     rewrite upd_ne; eauto;
+     apply H0; eauto].
+
+    destruct (handle_eq_dec h h0); subst;
+    [rewrite upd_eq in H1; eauto; cleanup;
+     repeat rewrite upd_eq; eauto |
+     rewrite upd_ne in H1; eauto;
+     repeat rewrite upd_ne; eauto;
+     apply H0; eauto].
+  }
+Qed.
+
+Lemma combine_length_eq_refl_l:
+  forall T1 T2 (l1: list T1) (l2: list T2) l3 l4,
+    combine l1 l2 = combine l3 l4 ->
+    length l1 = length l2 ->
+    length l3 = length l4 ->
+    l1 = l3.
+Proof.
+  induction l1; intros; simpl in *.
+  destruct l3; eauto.
+  destruct l4; simpl in *; congruence.
+  destruct l2; simpl in *; try congruence.
+  destruct l3; simpl in *; try congruence.
+  destruct l4; simpl in *; try congruence.
+  inversion H; subst.
+  erewrite IHl1; eauto. 
+Qed.
+
+Lemma combine_length_eq_refl_r:
+  forall T1 T2 (l2: list T2) (l1: list T1)  l3 l4,
+    combine l1 l2 = combine l3 l4 ->
+    length l1 = length l2 ->
+    length l3 = length l4 ->
+    l2 = l4.
+Proof.
+  induction l2; intros; simpl in *.
+  destruct l4; eauto.
+  rewrite ListUtils.combine_l_nil in H.
+  destruct l3; simpl in *; try congruence.
+  destruct l1; simpl in *; try congruence.
+  destruct l4; simpl in *; try congruence.
+  rewrite ListUtils.combine_l_nil in H; congruence.
+  destruct l3; simpl in *; try congruence.
+  inversion H; subst.
+  erewrite IHl2; eauto. 
+Qed.
+
+Lemma combine_length_eq_refl:
+  forall T1 T2 (l2: list T2) (l1: list T1)  l3 l4,
+    combine l1 l2 = combine l3 l4 ->
+    length l1 = length l2 ->
+    length l3 = length l4 ->
+    l1 = l3 /\ l2 = l4.
+Proof.
+  intros; split.
+  eapply combine_length_eq_refl_l; eauto.
+  eapply combine_length_eq_refl_r; eauto.
+Qed.
+
+Lemma disk_merges_to_upd:
+  forall V1 V2 (dt: @mem addr addr_eq_dec (V1 * list V1)) (d: @mem addr addr_eq_dec (V2 * list V2)) dtb a x1 x2 l1 l2,
+    (disk_merges_to (AEQ:= addr_eq_dec)) dt d dtb ->
+    length l1 = length l2 ->
+    (disk_merges_to (AEQ:= addr_eq_dec)) (upd dt a (x1, l1)) (upd d a (x2, l2)) ((upd (AEQ:=addr_eq_dec)) dtb a ((x1,x2), combine l1 l2)).
+Proof.
+  unfold disk_merges_to, diskmatch; intros.
+  cleanup.
+  split; intros.
+  {
+     destruct (addr_eq_dec a a0); subst.
+     repeat rewrite upd_eq; eauto.
+     right; do 2 eexists; eauto.
+     repeat rewrite upd_ne; eauto.
+  }
+  {
+    split; intros; cleanup.
+    destruct (addr_eq_dec a a0); subst;
+    [rewrite upd_eq in H2; eauto;
+     rewrite upd_eq in H3; eauto; cleanup;
+     rewrite upd_eq; eauto |
+     rewrite upd_ne in H2; eauto;
+     rewrite upd_ne in H3; eauto;
+     rewrite upd_ne; eauto;
+     apply H1; eauto].
+
+    destruct (addr_eq_dec a a0); subst;
+    [rewrite upd_eq in H2; eauto; cleanup;
+     repeat rewrite upd_eq; eauto |
+     rewrite upd_ne in H2; eauto;
+     repeat rewrite upd_ne; eauto;
+     apply H1; eauto].
+    destruct ts, bs; simpl in *.
+    apply combine_length_eq_refl in H7; eauto; cleanup; eauto.
+    
+  }
+Qed.
+
+
+Lemma disk_merges_to_some_eq:
+  forall V1 V2 (dt: @mem addr addr_eq_dec (V1 * list V1)) (d: @mem addr addr_eq_dec (V2 * list V2))
+    dtb a x1 x2 x3,
+    (disk_merges_to (AEQ:= addr_eq_dec)) dt d dtb ->
+    dt a = Some x1 ->
+    d a = Some x2 ->
+    dtb a = Some x3 ->
+    x3 = (fst x1, fst x2, combine (snd x1) (snd x2)).
+Proof.
+  unfold disk_merges_to, diskmatch; intros.
+  cleanup; specialize (H3 a x1 x2); destruct H3.  
+  destruct H3; eauto. rewrite H3 in H2; cleanup; eauto.
+Qed.
+
+
+Lemma mem_merges_to_some_eq:
+  forall V1 V2 (bm: block_mem V1) (bt: block_mem V2) btb h x1 x2 x3,
+    (mem_merges_to (AEQ:= handle_eq_dec)) bt bm btb ->
+    bt h = Some x1 ->
+    bm h = Some x2 ->
+    btb h = Some x3 ->
+    x3 = (x1, x2).
+Proof.
+  unfold mem_merges_to, memmatch; intros.
+  cleanup; specialize (H3 h); edestruct H3.
+  destruct (btb h); try congruence; cleanup.
+  destruct x3; simpl in *.
+  assert (A: bt h = Some x1 /\ bm h = Some x2).
+  eauto.
+  specialize (H4 A); cleanup; auto.
+Qed.
+
+
+Lemma combine_split_length :
+  forall T1 T2 (l1: list T1) (l2: list T2),
+    split (combine l1 l2) = (l1, l2) ->
+    length l1 = length l2.
+Proof.
+  induction l1; intros; simpl in *.
+  inversion H; simpl in *; subst; eauto.
+  destruct l2; simpl in *; try congruence.
+  erewrite IHl1; eauto.
+  destruct (split (combine l1 l2)); inversion H; eauto.
+Qed.
+
+Lemma disk_merges_to_none:
+  forall V1 V2 (dt: @mem addr addr_eq_dec (V1 * list V1)) (d: @mem addr addr_eq_dec (V2 * list V2))
+    dtb a,
+    (disk_merges_to (AEQ:= addr_eq_dec)) dt d dtb ->
+    dt a = None \/ d a = None ->
+    dtb a = None.
+Proof.
+  unfold disk_merges_to, diskmatch; intros.
+  cleanup; specialize (H1 a); specialize (H a).
+  destruct H; cleanup.
+  clear H0. destruct (dtb a); eauto.
+  edestruct p, p0, H1.
+  edestruct H3; eauto; cleanup.
+  eassign (v, fst (split l));
+    eassign (v0, snd (split l)); simpl.
+  pose proof (split_combine l).
+  destruct (split l) eqn:D; simpl in *; cleanup; eauto.
+  apply combine_split_length in D; eauto.
+  congruence.
+  split_ors; congruence.
+Qed.
+
+Lemma disk_merges_to_some_length:
+  forall V1 V2 (dt: @mem addr addr_eq_dec (V1 * list V1)) (d: @mem addr addr_eq_dec (V2 * list V2))
+    dtb a x1 x2,
+    (disk_merges_to (AEQ:= addr_eq_dec)) dt d dtb ->
+    dt a = Some x1 ->
+    d a = Some x2 ->
+    length (vsmerge x1) = length (vsmerge x2).
+Proof.
+  unfold disk_merges_to, diskmatch; intros.
+  cleanup; specialize (H a).
+  destruct H; cleanup; try congruence.
+  destruct x1, x2; simpl in *; eauto.
+Qed.
+
+Lemma combine_nil_either:
+  forall T1 T2 (l1: list T1) (l2: list T2),
+    combine l1 l2 = nil ->
+    l1 = nil \/ l2 = nil.
+Proof.
+  intros; destruct l1; eauto; destruct l2; eauto; simpl in *; congruence.
+Qed.
+
+Lemma disk_merges_to_sync_mem:
+  forall V1 V2 (dt: @mem addr addr_eq_dec (V1 * list V1)) (d: @mem addr addr_eq_dec (V2 * list V2)) (dtb: @mem addr addr_eq_dec ((V1 * V2) * list (V1 * V2))),
+    (disk_merges_to (AEQ:= addr_eq_dec)) dt d dtb ->
+    (disk_merges_to (AEQ:= addr_eq_dec)) (sync_mem dt) (sync_mem d) (sync_mem dtb).
+Proof.
+  unfold disk_merges_to, diskmatch, sync_mem; intros.
+  cleanup.
+  split; intros.
+  {
+    specialize (H a); split_ors; cleanup; eauto.
+    destruct x, x0; right; do 2 eexists; eauto.
+  }
+  {
+    specialize (H0 a).
+    split; intros; cleanup; try congruence;
+    edestruct H0.
+    edestruct H1; eauto.
+    rewrite H3; eauto.
+    edestruct H3; eauto.
+    eassign (fst ts, fst (split l));
+    eassign (fst bs, snd (split l)); simpl.
+    pose proof (split_combine l).
+    destruct (split l) eqn:D0; simpl in *; cleanup; eauto.
+    split; eauto.
+    apply combine_split_length in D0; eauto.
+    destruct ts, bs; simpl in *; cleanup; eauto.
+    symmetry in H5; apply combine_nil_either in H5; split_ors; cleanup; simpl in *.
+    symmetry in H2; apply length_zero_iff_nil in H2; cleanup; eauto.
+    apply length_zero_iff_nil in H2; cleanup; eauto.
+  }
+Qed.
+
+
+
+
+
 
 Lemma read_secure:
   forall pr a,
@@ -85,51 +347,74 @@ Lemma read_secure:
      >} Read a.
 Proof.
   unfold corr2; intros.
-  destruct_lift H; cleanup.
+  destruct_lift H1; cleanup.
   repeat inv_exec_perm; simpl in *; cleanup;
   try rewrite app_nil_r.
   {
-    edestruct H4; eauto.
-    pred_apply; cancel; eauto.
-    apply ptsto_subset_valid' in H; cleanup; eauto.
+    edestruct H6.
+    4: eauto.
+    all: eauto.
+    eapply mem_merges_to_upd; eauto.
+    pred_apply; cancel; eauto.    
+    eapply mem_merges_to_none; eauto.      
+    apply ptsto_subset_valid' in H1; cleanup; eauto; simpl in *.
+    eapply disk_merges_to_some_eq in H; eauto; cleanup.
+    inversion H; cleanup; eauto.
+    apply block_mem_subset_upd_none; eauto.
+    eapply mem_merges_to_none; eauto.
   }
   split_ors; cleanup.
   {
     split.
-    right; do 3 eexists; intuition.
-    inv_exec_perm.
-    apply H3.
+    right; do 6 eexists; intuition.
+    inv_exec_perm; eauto.
+    inv_exec_perm; eauto.
+    eapply H5.
     pred_apply; cancel; eauto.
     inv_exec_perm; cleanup; simpl; auto.
   }
   {
-    split.
-    right; eexists; intuition.
     inv_exec_perm.
-    edestruct H4; eauto.
-    pred_apply; cancel; eauto.
-    apply ptsto_subset_valid' in H; cleanup; eauto.
+    edestruct H6.
+    4: eauto.
+    all: eauto.
+    eapply mem_merges_to_upd; eauto.
+    pred_apply; cancel; eauto.    
+    eapply mem_merges_to_none; eauto.      
+    apply ptsto_subset_valid' in H1; cleanup; eauto; simpl in *.
+    eapply disk_merges_to_some_eq in H; eauto; cleanup.
+    inversion H; cleanup; eauto.
+    apply block_mem_subset_upd_none; eauto.
+    eapply mem_merges_to_none; eauto.
+    split.
+    right.
     split_ors; cleanup; try congruence.
-    do 2 eexists; intuition eauto.
-    inv_exec_perm; cleanup; auto.
-    try rewrite app_nil_r.
-    edestruct H4; eauto.
-    pred_apply; cancel; eauto.
-    apply ptsto_subset_valid' in H; cleanup; eauto.
+    do 6 eexists; intuition eauto.
+    try rewrite app_nil_r; eauto.
   }
   split_ors; cleanup.
   {
     inv_exec_perm.
-    apply ptsto_subset_valid' in H; cleanup; congruence.
+    apply ptsto_subset_valid' in H1; cleanup.
+    eapply disk_merges_to_none in H; eauto; cleanup; congruence.    
   }
   {
     repeat inv_exec_perm; simpl in *; cleanup.
     try rewrite app_nil_r.
-    edestruct H4; eauto.
-    pred_apply; cancel; eauto.
-    apply ptsto_subset_valid' in H; cleanup; eauto.
+    edestruct H6.
+    4: eauto.
+    all: eauto.
+    eapply mem_merges_to_upd; eauto.
+    pred_apply; cancel; eauto.    
+    eapply mem_merges_to_none; eauto.      
+    apply ptsto_subset_valid' in H1; cleanup; eauto; simpl in *.
+    eapply disk_merges_to_some_eq in H; eauto; cleanup.
+    inversion H; cleanup; eauto.
+    apply block_mem_subset_upd_none; eauto.
+    eapply mem_merges_to_none; eauto.
   }
 Qed.
+
 
 Lemma write_secure:
   forall pr a i,
@@ -145,63 +430,76 @@ Lemma write_secure:
      >} Write a i.
 Proof.
   unfold corr2; intros.
-  destruct_lift H; cleanup.
+  destruct_lift H1; cleanup.
   repeat inv_exec_perm; simpl in *; cleanup;
   try rewrite app_nil_r.
   {
-    edestruct H4; eauto.
-    apply ptsto_subset_valid' in H as Hx; cleanup; eauto.
-    eapply ptsto_subset_upd  with (v:= tb)(vs':= vsmerge (dummy1_cur, x)) in H.
-    pred_apply; cancel; eauto.
+    edestruct H6.
+    4: eauto.
+    all: eauto.
+    apply disk_merges_to_upd; eauto.
+    eapply disk_merges_to_some_length; eauto.
+    apply ptsto_subset_valid' in H1 as Hx; cleanup; eauto.
+    eapply disk_merges_to_some_eq in H as Hx; eauto; simpl in *.
+    eapply mem_merges_to_some_eq in H0 as Hy; eauto; simpl in *.
+    inversion Hx; cleanup; clear Hx.
+    eapply ptsto_subset_upd  with (v:= (t2, b1))(vs':= (fst ts, fst bs) :: combine (snd ts) (snd bs)) in H1.
+    pred_apply; cancel; eauto.    
     unfold vsmerge; simpl;
-    apply ListUtils.incl_cons2; auto.
+    apply ListUtils.incl_cons2; eauto.
   }
   split_ors; cleanup.
   {
-    split.
-    right; eexists; intuition.
     inv_exec_perm.
-    do 2 eexists; intuition eauto.
-    apply H3.
+    split; simpl; eauto.
+    right; do 6 eexists; intuition eauto.
+    eapply H5.
     pred_apply; cancel; eauto.
-    inv_exec_perm; cleanup; simpl; auto.
   }
   {
-    split.
-    right; eexists; intuition.
     inv_exec_perm.
-    edestruct H4; eauto.
-    apply ptsto_subset_valid' in H as Hx; cleanup; eauto.
-    eapply ptsto_subset_upd  with (v:= tb)(vs':= vsmerge (dummy1_cur, x)) in H as Hy.
-    pred_apply; cancel; eauto.
+    edestruct H6.
+    4: eauto.
+    all: eauto.
+    apply disk_merges_to_upd; eauto.
+    eapply disk_merges_to_some_length; eauto.
+    apply ptsto_subset_valid' in H1 as Hx; cleanup; eauto.
+    eapply disk_merges_to_some_eq in H as Hx; eauto; simpl in *.
+    eapply mem_merges_to_some_eq in H0 as Hy; eauto; simpl in *.
+    inversion Hx; cleanup; clear Hx.
+    eapply ptsto_subset_upd  with (v:= (t1, b1))(vs':= (fst ts, fst bs) :: combine (snd ts) (snd bs)) in H1.
+    pred_apply; cancel; eauto.    
     unfold vsmerge; simpl;
-    apply ListUtils.incl_cons2; auto.
-    split_ors; cleanup; try congruence.
-    do 2 eexists; intuition eauto.
-    inv_exec_perm; cleanup; simpl; auto.
+    apply ListUtils.incl_cons2; eauto.
     try rewrite app_nil_r.
-    edestruct H4; eauto.
-    apply ptsto_subset_valid' in H as Hx; cleanup; eauto.
-    eapply ptsto_subset_upd  with (v:= tb)(vs':= vsmerge (dummy1_cur, x)) in H.
-    pred_apply; cancel; eauto.
-    unfold vsmerge; simpl;
-    apply ListUtils.incl_cons2; auto.
+    split_ors; cleanup; try congruence.
+    split; eauto.
+    right; do  6 eexists; cleanup; eauto.
   }
   split_ors; cleanup.
   {
     inv_exec_perm; cleanup.
-    apply ptsto_subset_valid' in H as Hx; cleanup; eauto.
-    intuition congruence.
+    apply ptsto_subset_valid' in H1 as Hx; cleanup; eauto.
+    split_ors.
+    eapply mem_merges_to_none in H0; eauto; congruence.
+    eapply disk_merges_to_none in H; eauto; congruence.
   }
   {
     inv_exec_perm; cleanup;
-    try rewrite app_nil_r.
-    edestruct H4; eauto.
-    apply ptsto_subset_valid' in H as Hx; cleanup; eauto.
-    eapply ptsto_subset_upd  with (v:= tb)(vs':= vsmerge (dummy1_cur, x)) in H.
-    pred_apply; cancel; eauto.
+      try rewrite app_nil_r.
+    edestruct H6.
+    4: eauto.
+    all: eauto.
+    apply disk_merges_to_upd; eauto.
+    eapply disk_merges_to_some_length; eauto.
+    apply ptsto_subset_valid' in H1 as Hx; cleanup; eauto.
+    eapply disk_merges_to_some_eq in H as Hx; eauto; simpl in *.
+    eapply mem_merges_to_some_eq in H0 as Hy; eauto; simpl in *.
+    inversion Hx; cleanup; clear Hx.
+    eapply ptsto_subset_upd  with (v:= (t, b0))(vs':= (fst ts, fst bs) :: combine (snd ts) (snd bs)) in H1.
+    pred_apply; cancel; eauto.    
     unfold vsmerge; simpl;
-    apply ListUtils.incl_cons2; auto.
+    apply ListUtils.incl_cons2; eauto.
   }
 Qed.
 
@@ -221,29 +519,45 @@ Lemma seal_secure:
      >!} Seal t b.
 Proof.
   unfold corr2; intros.
-  destruct_lift H; cleanup.
+  destruct_lift H1; cleanup.
   repeat inv_exec_perm; simpl in *; cleanup.
   {
-    edestruct H4; eauto.
-    pred_apply; cancel; eauto.  
+    edestruct H6.
+    4: eauto.
+    all: eauto.
+    eapply mem_merges_to_upd; eauto.
+    pred_apply; cancel; eauto.    
+    eapply mem_merges_to_none; eauto.      
+    apply block_mem_subset_upd_none; eauto.
+    eapply mem_merges_to_none; eauto.
+    rewrite app_nil_r.
     split; auto.
-    apply only_public_operations_app_merge; simpl; auto.
   }
   split_ors; cleanup; inv_exec_perm.
   {
-    edestruct H4; eauto.
-    pred_apply; cancel; eauto.
-    split_ors; cleanup; try congruence.
-    split.
-    right; do 3 eexists; intuition.
-    apply only_public_operations_app_merge; simpl; auto.
+    edestruct H6.
+    4: eauto.
+    all: eauto.
+    eapply mem_merges_to_upd; eauto.
+    pred_apply; cancel; eauto.    
+    eapply mem_merges_to_none; eauto.      
+    apply block_mem_subset_upd_none; eauto.
+    eapply mem_merges_to_none; eauto.
+    rewrite app_nil_r.
+    split; auto.
   }
   split_ors; cleanup; inv_exec_perm.
   {
-    edestruct H4; eauto.
-    pred_apply; cancel; eauto.  
+    edestruct H6.
+    4: eauto.
+    all: eauto.
+    eapply mem_merges_to_upd; eauto.
+    pred_apply; cancel; eauto.    
+    eapply mem_merges_to_none; eauto.      
+    apply block_mem_subset_upd_none; eauto.
+    eapply mem_merges_to_none; eauto.
+    rewrite app_nil_r.
     split; auto.
-    apply only_public_operations_app_merge; simpl; auto.
   }
 Qed.
 
@@ -263,29 +577,45 @@ Lemma seal_secure_weak:
      W>!} Seal t b.
 Proof.
   unfold corr2_weak; intros.
-  destruct_lift H; cleanup.
+  destruct_lift H1; cleanup.
   repeat inv_exec_perm; simpl in *; cleanup.
   {
-    edestruct H4; eauto.
-    pred_apply; cancel; eauto.  
+    edestruct H6.
+    4: eauto.
+    all: eauto.
+    eapply mem_merges_to_upd; eauto.
+    pred_apply; cancel; eauto.    
+    eapply mem_merges_to_none; eauto.      
+    apply block_mem_subset_upd_none; eauto.
+    eapply mem_merges_to_none; eauto.
+    rewrite app_nil_r.
     split; auto.
-    apply trace_secure_app; simpl; auto.
   }
   split_ors; cleanup; inv_exec_perm.
   {
-    edestruct H4; eauto.
-    pred_apply; cancel; eauto.
-    split_ors; cleanup; try congruence.
-    split.
-    right; do 3 eexists; intuition.
-    apply trace_secure_app; simpl; auto.
+    edestruct H6.
+    4: eauto.
+    all: eauto.
+    eapply mem_merges_to_upd; eauto.
+    pred_apply; cancel; eauto.    
+    eapply mem_merges_to_none; eauto.      
+    apply block_mem_subset_upd_none; eauto.
+    eapply mem_merges_to_none; eauto.
+    rewrite app_nil_r.
+    split; auto.
   }
   split_ors; cleanup; inv_exec_perm.
   {
-    edestruct H4; eauto.
-    pred_apply; cancel; eauto.  
+    edestruct H6.
+    4: eauto.
+    all: eauto.
+    eapply mem_merges_to_upd; eauto.
+    pred_apply; cancel; eauto.    
+    eapply mem_merges_to_none; eauto.      
+    apply block_mem_subset_upd_none; eauto.
+    eapply mem_merges_to_none; eauto.
+    rewrite app_nil_r.
     split; auto.
-    apply trace_secure_app; simpl; auto.
   }
 Qed.
 
@@ -304,31 +634,48 @@ Lemma unseal_secure:
      >!} Unseal i.
 Proof.
   unfold corr2; intros.
-  destruct_lift H; cleanup.
+  destruct_lift H1; cleanup.
   repeat inv_exec_perm; simpl in *; cleanup.
   {
-    edestruct H4; eauto.
+    edestruct H6.
+    4: eauto.
+    all: eauto.
     pred_apply; cancel; eauto.
+    eapply mem_merges_to_some_eq in H0; eauto.
+    inversion H0; eauto.
     split; auto.
     apply only_public_operations_app_merge; simpl; auto.
+    eapply mem_merges_to_some_eq in H0; eauto.
+    inversion H0; eauto.
   }
   split_ors; cleanup; inv_exec_perm.
   {
-    edestruct H4; eauto.
-    cleanup.
+    edestruct H6.
+    4: eauto.
+    all: eauto.
     pred_apply; cancel; eauto.
-    split_ors; cleanup; try congruence.
-    split.
-    right; do 3 eexists; intuition.
+    eapply mem_merges_to_some_eq in H0; eauto.
+    inversion H0; eauto.
+    split; auto.
     apply only_public_operations_app_merge; simpl; auto.
+    eapply mem_merges_to_some_eq in H0; eauto.
+    inversion H0; eauto.
   }
   split_ors; cleanup; inv_exec_perm; try congruence.
   {
-    cleanup.
-    edestruct H4; eauto.
+    eapply mem_merges_to_none in H0; eauto; congruence.
+  }
+  {
+    edestruct H6.
+    4: eauto.
+    all: eauto.
     pred_apply; cancel; eauto.
+    eapply mem_merges_to_some_eq in H0; eauto.
+    inversion H0; eauto.
     split; auto.
     apply only_public_operations_app_merge; simpl; auto.
+    eapply mem_merges_to_some_eq in H0; eauto.
+    inversion H0; eauto.
   }
 Qed.
 
@@ -348,31 +695,48 @@ Lemma unseal_secure_weak:
      W>!} Unseal i.
 Proof.
   unfold corr2_weak; intros.
-  destruct_lift H; cleanup.
+  destruct_lift H1; cleanup.
   repeat inv_exec_perm; simpl in *; cleanup.
   {
-    edestruct H4; eauto.
+    edestruct H6.
+    4: eauto.
+    all: eauto.
     pred_apply; cancel; eauto.
+    eapply mem_merges_to_some_eq in H0; eauto.
+    inversion H0; eauto.
     split; auto.
-    apply trace_secure_app; simpl; auto.
+    apply trace_secure_app; simpl; eauto.
+    eapply mem_merges_to_some_eq in H0; eauto.
+    inversion H0; cleanup; eauto.
   }
   split_ors; cleanup; inv_exec_perm.
   {
-    edestruct H4; eauto.
-    cleanup.
+    edestruct H6.
+    4: eauto.
+    all: eauto.
     pred_apply; cancel; eauto.
-    split_ors; cleanup; try congruence.
-    split.
-    right; do 3 eexists; intuition.
-    apply trace_secure_app; simpl; auto.
+    eapply mem_merges_to_some_eq in H0; eauto.
+    inversion H0; eauto.
+    split; auto.
+    apply trace_secure_app; simpl; eauto.
+    eapply mem_merges_to_some_eq in H0; eauto.
+    inversion H0; cleanup; eauto.
   }
   split_ors; cleanup; inv_exec_perm; try congruence.
   {
-    cleanup.
-    edestruct H4; eauto.
+    eapply mem_merges_to_none in H0; eauto; congruence.
+  }
+  {
+    edestruct H6.
+    4: eauto.
+    all: eauto.
     pred_apply; cancel; eauto.
+    eapply mem_merges_to_some_eq in H0; eauto.
+    inversion H0; eauto.
     split; auto.
-    apply trace_secure_app; simpl; auto.
+    apply trace_secure_app; simpl; eauto.
+    eapply mem_merges_to_some_eq in H0; eauto.
+    inversion H0; cleanup; eauto.
   }
 Qed.
 
@@ -390,23 +754,29 @@ Lemma ret_secure:
      >!} Ret v.
 Proof.
   unfold corr2; intros.
-  destruct_lift H; cleanup.
+  destruct_lift H1; cleanup.
   repeat inv_exec_perm; simpl in *; cleanup;
   try rewrite app_nil_r.
   {
-    edestruct H4; eauto.
+     edestruct H6.
+     4: eauto.
+     all: eauto.
+     pred_apply; cancel; eauto.
+  }
+  split_ors; cleanup; inv_exec_perm;
+  try rewrite app_nil_r.
+  {
+     edestruct H6.
+    4: eauto.
+    all: eauto.
     pred_apply; cancel; eauto.
   }
   split_ors; cleanup; inv_exec_perm;
   try rewrite app_nil_r.
   {
-    edestruct H4; eauto.
-    pred_apply; cancel; eauto.
-  }
-  split_ors; cleanup; inv_exec_perm;
-  try rewrite app_nil_r.
-  {
-    edestruct H4; eauto.
+     edestruct H6.
+    4: eauto.
+    all: eauto.
     pred_apply; cancel; eauto.
   }
 Qed.
@@ -425,23 +795,29 @@ Lemma ret_secure_weak:
      W>!} Ret v.
 Proof.
   unfold corr2_weak; intros.
-  destruct_lift H; cleanup.
+  destruct_lift H1; cleanup.
   repeat inv_exec_perm; simpl in *; cleanup;
   try rewrite app_nil_r.
   {
-    edestruct H4; eauto.
+     edestruct H6.
+    4: eauto.
+    all: eauto.
     pred_apply; cancel; eauto.
   }
   split_ors; cleanup; inv_exec_perm;
   try rewrite app_nil_r.
   {
-    edestruct H4; eauto.
+     edestruct H6.
+    4: eauto.
+    all: eauto.
     pred_apply; cancel; eauto.
   }
   split_ors; cleanup; inv_exec_perm;
   try rewrite app_nil_r.
   {
-    edestruct H4; eauto.
+     edestruct H6.
+    4: eauto.
+    all: eauto.
     pred_apply; cancel; eauto.
   }
 Qed.
@@ -460,23 +836,29 @@ Lemma ret_secure':
      >!} Ret v.
 Proof.
   unfold corr2; intros.
-  destruct_lift H; cleanup.
+  destruct_lift H1; cleanup.
   repeat inv_exec_perm; simpl in *; cleanup;
   try rewrite app_nil_r.
   {
-    edestruct H4; eauto.
+     edestruct H6.
+    4: eauto.
+    all: eauto.
     pred_apply; cancel; eauto.
   }
   split_ors; cleanup; inv_exec_perm;
   try rewrite app_nil_r.
   {
-    edestruct H4; eauto.
+     edestruct H6.
+    4: eauto.
+    all: eauto.
     pred_apply; cancel; eauto.
   }
   split_ors; cleanup; inv_exec_perm;
   try rewrite app_nil_r.
   {
-    edestruct H4; eauto.
+     edestruct H6.
+    4: eauto.
+    all: eauto.
     pred_apply; cancel; eauto.
   }
 Qed.
@@ -495,11 +877,14 @@ Lemma sync_secure:
      >!} Sync.
 Proof.
   unfold corr2; intros.
-  destruct_lift H; cleanup.
+  destruct_lift H1; cleanup.
   repeat inv_exec_perm; simpl in *; cleanup;
   try rewrite app_nil_r.
   {
-    edestruct H4; eauto.
+    edestruct H6.
+    4: eauto.
+    all: eauto.
+    apply disk_merges_to_sync_mem; eauto.
     repeat rewrite <- sep_star_assoc.
     repeat (apply sep_star_lift_apply'; eauto).
     apply sep_star_comm; apply emp_star_r.
@@ -507,34 +892,31 @@ Proof.
   }
   split_ors; cleanup.
   {
-    split.
-    right; do 3 eexists; intuition.
     inv_exec_perm.
-    apply H3; pred_apply; cancel; eauto.
-    inv_exec_perm; cleanup; simpl; auto.
+    split.
+    right; do 6 eexists; intuition eauto.
+    eapply H5; pred_apply; cancel; eauto.
+    simpl; auto.
   }
   {
-    split.
-    right; do 3 eexists; intuition.
     inv_exec_perm.
-    edestruct H4; eauto.
+    edestruct H6.
+    4: eauto.
+    all: eauto.
+    apply disk_merges_to_sync_mem; eauto.
     repeat rewrite <- sep_star_assoc.
     repeat (apply sep_star_lift_apply'; eauto).
     apply sep_star_comm; apply emp_star_r.
     apply sync_xform_pred_apply; auto.
-    split_ors; cleanup; try congruence.
-    inv_exec_perm; cleanup; auto.
-    try rewrite app_nil_r.
-    edestruct H4; eauto.
-    repeat rewrite <- sep_star_assoc.
-    repeat (apply sep_star_lift_apply'; eauto).
-    apply sep_star_comm; apply emp_star_r.
-    apply sync_xform_pred_apply; auto.
+    try rewrite app_nil_r; eauto.
   }
   split_ors; cleanup; inv_exec_perm;
   try rewrite app_nil_r.
   {
-    edestruct H4; eauto.
+    edestruct H6.
+    4: eauto.
+    all: eauto.
+    apply disk_merges_to_sync_mem; eauto.
     repeat rewrite <- sep_star_assoc.
     repeat (apply sep_star_lift_apply'; eauto).
     apply sep_star_comm; apply emp_star_r.
@@ -555,12 +937,15 @@ Lemma sync_secure':
          (F bm'' hm'')
      >!} Sync.
 Proof.
-  unfold corr2; intros.
-  destruct_lift H; cleanup.
+    unfold corr2; intros.
+  destruct_lift H1; cleanup.
   repeat inv_exec_perm; simpl in *; cleanup;
   try rewrite app_nil_r.
   {
-    edestruct H4; eauto.
+    edestruct H6.
+    4: eauto.
+    all: eauto.
+    apply disk_merges_to_sync_mem; eauto.
     repeat rewrite <- sep_star_assoc.
     repeat (apply sep_star_lift_apply'; eauto).
     apply sep_star_comm; apply emp_star_r.
@@ -568,34 +953,31 @@ Proof.
   }
   split_ors; cleanup.
   {
-    split.
-    right; do 3 eexists; intuition.
     inv_exec_perm.
-    apply H3; pred_apply; cancel; eauto.
-    inv_exec_perm; cleanup; simpl; auto.
+    split.
+    right; do 6 eexists; intuition eauto.
+    eapply H5; pred_apply; cancel; eauto.
+    simpl; auto.
   }
   {
-    split.
-    right; do 3 eexists; intuition.
     inv_exec_perm.
-    edestruct H4; eauto.
+    edestruct H6.
+    4: eauto.
+    all: eauto.
+    apply disk_merges_to_sync_mem; eauto.
     repeat rewrite <- sep_star_assoc.
     repeat (apply sep_star_lift_apply'; eauto).
     apply sep_star_comm; apply emp_star_r.
     apply sync_xform_pred_apply; auto.
-    split_ors; cleanup; try congruence.
-    inv_exec_perm; cleanup; auto.
-    try rewrite app_nil_r.
-    edestruct H4; eauto.
-    repeat rewrite <- sep_star_assoc.
-    repeat (apply sep_star_lift_apply'; eauto).
-    apply sep_star_comm; apply emp_star_r.
-    apply sync_xform_pred_apply; auto.
+    try rewrite app_nil_r; eauto.
   }
   split_ors; cleanup; inv_exec_perm;
   try rewrite app_nil_r.
   {
-    edestruct H4; eauto.
+    edestruct H6.
+    4: eauto.
+    all: eauto.
+    apply disk_merges_to_sync_mem; eauto.
     repeat rewrite <- sep_star_assoc.
     repeat (apply sep_star_lift_apply'; eauto).
     apply sep_star_comm; apply emp_star_r.
